% -----------------------------------------------
%     Einstellungen zum Layout:
% -----------------------------------------------
\documentclass[12pt,oneside,a4paper,parskip=on,fleqn]{scrartcl}
\usepackage[left=3cm,right=3cm,top=3cm,bottom=3cm,includehead]{geometry}
\usepackage{ngerman}
\usepackage[utf8]{inputenc}
\usepackage{amsmath}
\usepackage{amssymb}
\usepackage{xfrac}
\setlength\parindent{0pt}   % Festlegen des Absatzeinzuges

\begin{document}
\section*{Proof of Note 7}
\begin{enumerate}
	\item $f(u,v) = -f(v,u) \Rightarrow f(u,u) = 0$
	\item $\sum_{u\in V} f(u,v) = \sum_{u\in V} f(v,u) = 0$
	\item $(u,v),(v,u)\not\in E \Rightarrow c(u,v) = 0 = c(v,u)$\\
	$\Rightarrow f(u,v) \leq c(u,v) = 0,\quad f(v,u) \leq 0 \Rightarrow d)$
\end{enumerate}

\section*{Proof of Lemma 6}
a) $$2\cdot f(X,X) = \sum_{x\in X}\sum_{y\in X} f(x,y) + \sum_{y\in X} \sum_{x\in X} f(y,x)$$
$$=\sum_{x\in X}\sum_{y\in X} f(x,y) + f(y,x) = 0$$
b) $$f(X,Y) = \sum_{x\in X}\sum_{y\in Y} f(x,y)$$
$$=\sum_{x\in X}\sum_{y\in Y}-f(y,x)=-\sum_{y\in Y}\sum_{x\in X} f(y,x) = -f(Y,X)$$
c) $$f(X\cup Y,Z) = \sum_{x\in X} \sum_{z\in Z} f(x,z) + \sum_{y\in Y}\sum_{z\in Z} f(y,z) = f(X,Z) + f(Y,Z)$$

\section*{Proof of Lemma 7}
\begin{enumerate}
	\item Capacity constraints:
		$$(f+f')(u,v) = f(u,v) + f'(u,v)\leq f(u,v) + c_f(u,v)$$
		$$\leq f(u,v) + c(u,v) - f(u,v) = c(u,v)$$
	\item Skew symmetrie:
		$$(f+f')(u,v) = f(u,v) + f'(u,v) = -f(v,u) - f'(v,u) = -(f+f')(v,u)$$
	\item Flow conservation:
		$$\forall u\in V-\{s,t\} \text{ we have}$$
		$$\sum_{v\in V} (f+f')(u,v) = \sum_{v\in V} f(u,v) + \sum_{v\in V} f'(u,v) = 0$$
	\item $$|f+f'|= \sum_{v\in V}(f+f')(v,t)$$
	$$=\sum_{v\in V} f(v,t) + \sum_{v\in V} f'(v,t) = |f| + |f'|$$
\end{enumerate}

\section*{Proof of Lemma 8} % (fold)
\label{sec:proof_of_lemma_8}
\begin{enumerate}
	\item Capacity constraint:
		\[
			(u,v)\in P: f_P(u,v) = c_f(P) = \min\{c_f(u,v)| (u,v)\in P\}\leq (u,v)\]
			\[
			(u,v)\not\in P: f_P(u,v) \leq 0 \leq c(u,v)-f(u,v) = c_f(u,v)
		\]
	\item Skew symmetrie: clear
	\item Flow cons:
		\[
			u\not\in P: \sum_{v\in V} f_P(u,v) = 0\\
			u\in P: s\rightsquigarrow x\to u\to y\rightsquigarrow t
		\]
		\[
			\sum_{v\in V} f_P(u,v) = f_P(u,x) + f_P(u,y) \underset{\text{skew}}{=} f_P(u,y) - f_P(x,u) = c_f(P) - c_f(P) = 0
		\]
\end{enumerate}
% section proof_of_lemma_8 (end)
\end{document}